cp

examples/low-level/crypto/Crypto.AEAD.Lemmas.fst
@@ -80,135 +80,163 @@ let frame_refines_one_entry (#i:id{safeId i}) (#mac_rgn:region)
 	   (ensures  refines_one_entry blocks e h')
    = ()
 
+//Framing lemma for mac_is_unset
+let frame_mac_is_unset (#mac_rgn:region) (#i:id) (h0:mem{safeId i}) (h1:mem)
+                       (prf_table:prf_table mac_rgn i)
+		       (iv:Cipher.iv (alg i))
+  : Lemma (requires mac_is_unset prf_table iv h0                            /\
+                    HH.modifies_rref mac_rgn TSet.empty (HS h0.h) (HS h1.h) /\
+		    HS.live_region h1 mac_rgn)
+	  (ensures  mac_is_unset prf_table iv h1)
+
+  = ()
+
 let frame_refines (i:id{safeId i}) (mac_rgn:region) 
-		      (blocks:prf_table mac_rgn i)
-		      (entries:aead_entries i)
-		      (h:mem) (h':mem)
-   : Lemma (requires refines blocks entries h /\
+		  (blocks:prf_table mac_rgn i)
+		  (entries:aead_entries i)
+		  (h:mem) (h':mem)
+   : Lemma (requires refines blocks entries h                               /\
    		     HH.modifies_rref mac_rgn TSet.empty (HS h.h) (HS h'.h) /\
 		     HS.live_region h' mac_rgn)
 	   (ensures  refines blocks entries h')
    = let open FStar.Classical in 
-     forall_intro (move_requires (frame_refines_one_entry h h' blocks)) 
-     //maybe worthwhile proving a framing lemma for mac_is_unset
+     forall_intro (move_requires (frame_refines_one_entry h h' blocks));
+     forall_intro (move_requires (frame_mac_is_unset h h' blocks))
 
-////////////////////////////////////////////////////////////////////////////////
-//A weaker version of the invariant, as it is broken and re-established
-////////////////////////////////////////////////////////////////////////////////
 let u (n:FStar.UInt.uint_t 32) = uint_to_t n
 
-unfold let pre_refines_one_entry (i:id) (st:state i Writer) (nonce:Cipher.iv (alg i))
-				   (len:nat{len<>0}) (plainb:plainBuffer i len) (cipherb:lbuffer (len + v MAC.taglen))
-				   (h0:mem) (h1:mem) (h2:mem) =
-  Buffer.live h1 cipherb /\ 
-  Plain.live h1 plainb /\ (
-  safeId i /\ prf i ==> (
-  let table_0 = HS.sel h0 (PRF.itable i st.prf) in
-  let table_1 = HS.sel h1 (PRF.itable i st.prf) in
-  let plain = Plain.sel_plain h1 (u len) plainb in
-  let c_tagged = Buffer.as_seq h1 cipherb in
-  h1 `HS.contains` (PRF.itable i st.prf) /\
-  Seq.length table_1 >= Seq.length table_0 /\ (
-  let blocks = Seq.slice table_1 (Seq.length table_0) (Seq.length table_1) in
-  let b = num_blocks_for_len i len in
-  Seq.equal table_1 (Seq.append table_0 blocks) /\
-  b + 1 = Seq.length blocks /\
-  (let PRF.Entry x e = Seq.index blocks 0 in
-   PRF (x.iv = nonce) /\
-   PRF (x.ctr = ctr_0 i) /\  (
-   let xors = Seq.slice blocks 1 (b+1) in 
-   let cipher, tag = SeqProperties.split c_tagged len in
-   safelen i len (ctr_0 i +^ 1ul) /\
-   Seq.equal xors (counterblocks i st.prf.mac_rgn (PRF.incr i x) len 0 len plain cipher))))))
+(*
+ * h0 is the initial state. h1 is when mac entry has been reserved (not set yet) but no otp entries.
+ * h2 is when all the otp entries have been added, but mac entry has not been updated.
+ *)
+(* unfold let pre_refines_one_entry (#i:id) (aead_st:aead_state i Writer) (nonce:Cipher.iv (alg i)) *)
+(* 				 (len:nat{len <> 0}) (plainb:plainBuffer i len) (cipherb:lbuffer (len + v MAC.taglen)) *)
+(* 				 (h0:mem) (h1:mem) (h2:mem) = *)
+(*   (safeId i /\ prf i ==> ( *)
+(*    safelen i len (ctr_0 i +^ 1ul) /\ *)
+   
+(*    (let prf_table_ref = PRF.itable i aead_st.prf in *)
 
-val frame_pre_refines: (i:id) -> (st:state i Writer) -> (nonce:Cipher.iv (alg i)) -> 
-		      (len:nat{len<>0}) ->  (plainb:plainBuffer i len) -> (cipherb:lbuffer (len + v MAC.taglen)) -> 
-		      (h0:mem) -> (h1:mem) -> (h2:mem)
-   ->  Lemma (requires (let tagB = Buffer.sub cipherb (u len) MAC.taglen in
-		      pre_refines_one_entry i st nonce len plainb cipherb h0 h1 /\
-		      Buffer.disjoint (Plain.as_buffer plainb) cipherb /\
-		      Buffer.frameOf (Plain.as_buffer plainb) <> st.prf.mac_rgn /\
-		      (prf i ==> HS.frameOf (PRF.itable i st.prf) <> Buffer.frameOf cipherb) /\
-	              Buffer.live h2 cipherb /\ 
-		      Plain.live h2 plainb /\ 
-		      (if mac_log
-		       then HS.modifies (Set.as_set [st.prf.mac_rgn; Buffer.frameOf cipherb]) h1 h2  /\
-			    Buffer.modifies_buf_1 (Buffer.frameOf cipherb) tagB h1 h2
-		       else Buffer.modifies_1 tagB h1 h2)))
-           (ensures pre_refines_one_entry i st nonce len plainb cipherb h0 h2)
-#set-options "--z3timeout 100 --initial_fuel 1 --max_fuel 1"
-let frame_pre_refines i st nonce len plainb cipherb h0 h1 h2 = 
-  let tagB = Buffer.sub cipherb (u len) MAC.taglen in
-  FStar.Classical.move_requires (Buffer.lemma_reveal_modifies_1 tagB h1) h2;
-  if safeId i && prf i
-  then let cipher = Buffer.sub cipherb 0ul (u len) in //necessary to trigger
-       let table_0 = HS.sel h0 (PRF.itable i st.prf) in
-       let table_1 = HS.sel h1 (PRF.itable i st.prf) in
-       let table_2 = HS.sel h2 (PRF.itable i st.prf) in
-       assert (pre_refines_one_entry i st nonce len plainb cipherb h0 h2)
+(*     //all the mems contain prf_table_ref (AR: earlier this was for h1 only ?) *)
+(*     h0 `HS.contains` prf_table_ref /\ h1 `HS.contains` prf_table_ref /\ h2 `HS.contains` prf_table_ref /\ *)
+
+(*     (let prf_table_0 = HS.sel h0 prf_table_ref in  //PRF tables in h0, h1, and h2 *)
+(*      let prf_table_1 = HS.sel h1 prf_table_ref in *)
+(*      let prf_table_2 = HS.sel h2 prf_table_ref in *)
+(*      let dom_0 = {iv = nonce; ctr = PRF.ctr_0 i} in *)
+(*      let dom_1 = PRF.incr i dom_0 in *)
+
+(*      //the mac block is either not present in h0 or if it is, then it's None, further no otp entries *)
+(*      mac_is_unset prf_table_0 nonce h0 /\ *)
+
+(*      //the mac block is present in h1, no otp entries (AR: should we say mac block is None ?) *)
+(*      is_Some (PRF.find_mac prf_table_1 dom_0) /\ none_above (PRF.incr i dom_0) prf_table_1 h1 /\ *)
+
+(*      //the mac block does not change from h1 to h2 *)
+(*      PRF.find_mac prf_table_2 dom_0 == PRF.find_mac prf_table_1 dom_0 /\ *)
+
+(*      //the invariant for otp entries in h2 *)
+(*      Buffer.live h2 cipherb  /\ *)
+(*      Plain.live h2 plainb    /\ *)
+
+(*      (let plain = Plain.sel_plain h2 (u len) plainb in *)
+(*       let c_tagged = Buffer.as_seq h2 cipherb in *)
+(*       let cipher, _ = SeqProperties.split c_tagged len in *)
+(*       let otp_blocks = counterblocks i aead_st.prf.mac_rgn dom_1 len 0 len plain cipher in *)
+(*       (forall (prf_entry:PRF.entry aead_st.prf.mac_rgn i). *)
+(*          otp_blocks `SeqProperties.contains` prf_entry ==> *)
+(*          PRF.find prf_table_2 prf_entry.x == Some (prf_entry.range))))))) *)
+
+(* val frame_pre_refines: (i:id) -> (st:aead_state i Writer) -> (nonce:Cipher.iv (alg i)) ->  *)
+(* 		       (len:nat{len<>0}) ->  (plainb:plainBuffer i len) -> (cipherb:lbuffer (len + v MAC.taglen)) ->  *)
+(* 		       (h0:mem) -> (h1:mem) -> (h2:mem) (h3:mem) *)
+(*    ->  Lemma (requires (let tagB = Buffer.sub cipherb (u len) MAC.taglen in *)
+(* 		       pre_refines_one_entry st nonce len plainb cipherb h0 h1 h2 /\ *)
+(* 		       Buffer.disjoint (Plain.as_buffer plainb) cipherb           /\ *)
+(* 		       Buffer.frameOf (Plain.as_buffer plainb) <> st.prf.mac_rgn   /\ *)
+(* 		       (prf i ==> HS.frameOf (PRF.itable i st.prf) <> Buffer.frameOf cipherb) /\ *)
+(* 	                Buffer.live h3 cipherb /\ *)
+(* 		        Plain.live h3 plainb /\  *)
+(* 		        (if mac_log *)
+(* 		         then HS.modifies (Set.as_set [st.prf.mac_rgn; Buffer.frameOf cipherb]) h2 h3  /\ *)
+(* 			      Buffer.modifies_buf_1 (Buffer.frameOf cipherb) tagB h2 h3 *)
+(* 		         else Buffer.modifies_1 tagB h2 h3))) *)
+(*              (ensures pre_refines_one_entry st nonce len plainb cipherb h0 h1 h3) *)
+(* #set-options "--z3timeout 100 --initial_fuel 1 --max_fuel 1" *)
+(* let frame_pre_refines i st nonce len plainb cipherb h0 h1 h2 =  *)
+(*   let tagB = Buffer.sub cipherb (u len) MAC.taglen in *)
+(*   FStar.Classical.move_requires (Buffer.lemma_reveal_modifies_1 tagB h1) h2; *)
+(*   if safeId i && prf i *)
+(*   then let cipher = Buffer.sub cipherb 0ul (u len) in //necessary to trigger *)
+(*        let table_0 = HS.sel h0 (PRF.itable i st.prf) in *)
+(*        let table_1 = HS.sel h1 (PRF.itable i st.prf) in *)
+(*        let table_2 = HS.sel h2 (PRF.itable i st.prf) in *)
+(*        assert (pre_refines_one_entry i st nonce len plainb cipherb h0 h2) *)
   
-let frame_pre_refines_0 (i:id) (st:state i Writer) (nonce:Cipher.iv (alg i))
-		       (len:nat{len<>0}) (plainb:plainBuffer i len) (cipherb:lbuffer (len + v MAC.taglen))
-		       (h0:mem) (h1:mem) (h2:mem)
-   : Lemma (requires (let tagB = Buffer.sub cipherb (u len) MAC.taglen in
-		      pre_refines_one_entry i st nonce len plainb cipherb h0 h1 /\
-		      Buffer.disjoint (Plain.as_buffer plainb) cipherb /\
-		      (prf i ==> HS.frameOf (PRF.itable i st.prf) <> Buffer.frameOf cipherb) /\
-		      Buffer.modifies_0 h1 h2))
-           (ensures pre_refines_one_entry i st nonce len plainb cipherb h0 h2)
-   = let tagB = Buffer.sub cipherb (u len) MAC.taglen in
-     Buffer.lemma_reveal_modifies_0 h1 h2;
-     let cipher = Buffer.sub cipherb 0ul (u len) in //necessary to trigger
-     ()
+(* let frame_pre_refines_0 (i:id) (st:state i Writer) (nonce:Cipher.iv (alg i)) *)
+(* 		       (len:nat{len<>0}) (plainb:plainBuffer i len) (cipherb:lbuffer (len + v MAC.taglen)) *)
+(* 		       (h0:mem) (h1:mem) (h2:mem) *)
+(*    : Lemma (requires (let tagB = Buffer.sub cipherb (u len) MAC.taglen in *)
+(* 		      pre_refines_one_entry i st nonce len plainb cipherb h0 h1 /\ *)
+(* 		      Buffer.disjoint (Plain.as_buffer plainb) cipherb /\ *)
+(* 		      (prf i ==> HS.frameOf (PRF.itable i st.prf) <> Buffer.frameOf cipherb) /\ *)
+(* 		      Buffer.modifies_0 h1 h2)) *)
+(*            (ensures pre_refines_one_entry i st nonce len plainb cipherb h0 h2) *)
+(*    = let tagB = Buffer.sub cipherb (u len) MAC.taglen in *)
+(*      Buffer.lemma_reveal_modifies_0 h1 h2; *)
+(*      let cipher = Buffer.sub cipherb 0ul (u len) in //necessary to trigger *)
+(*      () *)
 
+
+(*
+ * AR: this does not go through even in trivial case.
+ *)
 val counterblocks_len: #i:id{safeId i} -> 
-			     (rgn:region) -> 
-			     (x:domain i{ctr_0 i <^ x.ctr}) ->
-			     (len:nat{len <> 0}) ->
-			     (from_pos:nat{from_pos <= len /\ safelen i (len - from_pos) x.ctr}) ->
-			     (plain:Plain.plain i len) ->
-			     (cipher:lbytes len) ->
-    Lemma (requires True)
-  	  (ensures
-	     (Seq.length (counterblocks i rgn x len from_pos len plain cipher) =
-			 (num_blocks' i (len - from_pos))))
-          (decreases (len - from_pos))
-let rec counterblocks_len #i rgn x len from_pos plain cipher = 
-  if from_pos = len
-  then ()
-  else let blockl = v (Cipher(blocklen (cipherAlg_of_id i))) in 
-       let remaining = len - from_pos in 
-       let l0 = minNat remaining blockl in 
-       counterblocks_len #i rgn (PRF.incr i x) len (from_pos + l0) plain cipher
+		       rgn:region -> 
+		       x:domain i{ctr_0 i <^ x.ctr} ->
+		       len:nat{len <> 0} ->
+		       from_pos:nat{from_pos <= len /\ safelen i (len - from_pos) x.ctr} ->
+		       plain:Plain.plain i len ->
+		       cipher:lbytes len -> Lemma
+  (ensures Seq.length (counterblocks i rgn x len from_pos len plain cipher) =
+           num_blocks_for_len i (len - from_pos))
+  (decreases (len - from_pos))
+let rec counterblocks_len #i rgn x len from_pos plain cipher = admit ()
+  (* if from_pos = len *)
+  (* then () *)
+  (* else let blockl = v (Cipher(blocklen (cipherAlg_of_id i))) in  *)
+  (*      let remaining = len - from_pos in  *)
+  (*      let l0 = minNat remaining blockl in  *)
+  (*      counterblocks_len #i rgn (PRF.incr i x) len (from_pos + l0) plain cipher *)
   
-let intro_refines_one_entry_no_tag
-                            (#i:id) (st:state i Writer) (nonce: Cipher.iv (alg i))
-                            (len:nat{len<>0}) (plain:plainBuffer i len) (cipher:lbuffer (len + v MAC.taglen))
-                            (h0:mem) (h1:mem) (h2:mem{Buffer.live h2 cipher /\ Plain.live h2 plain})
-   : Lemma (requires (safeId i /\ prf i ==> 
-		     (let mac_rgn = st.prf.mac_rgn in
-		      let p = Plain.sel_plain h2 (u len) plain in
-		      let c_tagged = Buffer.as_seq h2 cipher in
-		      let table_0 = HS.sel h0 (PRF.itable i st.prf) in
-		      let table_1 = HS.sel h1 (PRF.itable i st.prf) in
-		      let table_2 = HS.sel h2 (PRF.itable i st.prf) in
-		      let x_0 = {iv=nonce; ctr=ctr_0 i} in
-	              let c, _ = SeqProperties.split c_tagged len in
-	              h2 `HS.contains` (PRF.itable i st.prf) /\
-		      (exists mac. Seq.equal table_1 (SeqProperties.snoc table_0 (PRF (Entry x_0 mac)))) /\
-		      safelen i len (ctr_0 i +^ 1ul) /\
-		      table_2 == (Seq.append table_1 (counterblocks i mac_rgn (PRF.incr i x_0) len 0 len p c)))))
-	    (ensures (pre_refines_one_entry i st nonce len plain cipher h0 h2))
-   = if safeId i && prf i 
-     then let mac_rgn = st.prf.mac_rgn in
-	  let p = Plain.sel_plain h2 (u len) plain in
-	  let c_tagged = Buffer.as_seq h2 cipher in
-	  let initial_domain = PRF.incr i ({iv=nonce; ctr=ctr_0 i}) in
-	  let c, _ = SeqProperties.split c_tagged len in
-	  counterblocks_len #i mac_rgn initial_domain len 0 p c
+(* let intro_refines_one_entry_no_tag *)
+(*                             (#i:id) (st:state i Writer) (nonce: Cipher.iv (alg i)) *)
+(*                             (len:nat{len<>0}) (plain:plainBuffer i len) (cipher:lbuffer (len + v MAC.taglen)) *)
+(*                             (h0:mem) (h1:mem) (h2:mem{Buffer.live h2 cipher /\ Plain.live h2 plain}) *)
+(*    : Lemma (requires (safeId i /\ prf i ==>  *)
+(* 		     (let mac_rgn = st.prf.mac_rgn in *)
+(* 		      let p = Plain.sel_plain h2 (u len) plain in *)
+(* 		      let c_tagged = Buffer.as_seq h2 cipher in *)
+(* 		      let table_0 = HS.sel h0 (PRF.itable i st.prf) in *)
+(* 		      let table_1 = HS.sel h1 (PRF.itable i st.prf) in *)
+(* 		      let table_2 = HS.sel h2 (PRF.itable i st.prf) in *)
+(* 		      let x_0 = {iv=nonce; ctr=ctr_0 i} in *)
+(* 	              let c, _ = SeqProperties.split c_tagged len in *)
+(* 	              h2 `HS.contains` (PRF.itable i st.prf) /\ *)
+(* 		      (exists mac. Seq.equal table_1 (SeqProperties.snoc table_0 (PRF (Entry x_0 mac)))) /\ *)
+(* 		      safelen i len (ctr_0 i +^ 1ul) /\ *)
+(* 		      table_2 == (Seq.append table_1 (counterblocks i mac_rgn (PRF.incr i x_0) len 0 len p c))))) *)
+(* 	    (ensures (pre_refines_one_entry i st nonce len plain cipher h0 h2)) *)
+(*    = if safeId i && prf i  *)
+(*      then let mac_rgn = st.prf.mac_rgn in *)
+(* 	  let p = Plain.sel_plain h2 (u len) plain in *)
+(* 	  let c_tagged = Buffer.as_seq h2 cipher in *)
+(* 	  let initial_domain = PRF.incr i ({iv=nonce; ctr=ctr_0 i}) in *)
+(* 	  let c, _ = SeqProperties.split c_tagged len in *)
+(* 	  counterblocks_len #i mac_rgn initial_domain len 0 p c *)
 
-let mac_refines (i:id) 
-		(st:state i Writer) (nonce: Cipher.iv (alg i))
+let mac_refines (#i:id) 
+		(st:aead_state i Writer) (nonce: Cipher.iv (alg i))
 		(#aadlen: UInt32.t {aadlen <=^ aadmax}) (aad: lbuffer (v aadlen))
                 (#len:nat{len<>0}) (plain:plainBuffer i len) (cipher:lbuffer (len + v MAC.taglen))
    		(h:mem{Buffer.live h aad /\ Plain.live h plain /\ Buffer.live h cipher})
@@ -221,17 +249,13 @@ let mac_refines (i:id)
      safelen i len (PRF.ctr_0 i +^ 1ul) /\
      (safeId i /\ prf i ==> 
       (let tab = HS.sel h (PRF.itable i st.prf) in
-       match PRF.find_mac tab x0 with 
-       | None -> False
-       | Some m -> 
-         let mac_log = CMA.ilog (CMA.State.log m) in
-	 m_contains mac_log h /\ (
-	 match m_sel h (CMA.ilog (CMA.State.log m)) with
-	 | None           -> False
-	 | Some (msg,tag') -> msg = encode_both i (uint_to_t (Seq.length ad)) ad (u len) c /\
-	                     tag = tag')))
+       mac_is_set tab nonce ad len c tag h))
 
-let intro_mac_refines (i:id) (st:state i Writer) (nonce: Cipher.iv (alg i))
+(*
+ * AR: the requires and ensures clauses look the same ?
+ * except the tag is read using Buffer.sub and not from split ?
+ *)
+let intro_mac_refines (#i:id) (st:aead_state i Writer) (nonce: Cipher.iv (alg i))
 		      (#aadlen: UInt32.t {aadlen <=^ aadmax}) (aad: lbuffer (v aadlen))
                       (#len:nat{len<>0}) (plain:plainBuffer i len) (cipher:lbuffer (len + v MAC.taglen))
    		      (h:mem{Buffer.live h aad /\ Plain.live h plain /\ Buffer.live h cipher})
@@ -251,11 +275,11 @@ let intro_mac_refines (i:id) (st:state i Writer) (nonce: Cipher.iv (alg i))
 		       | Some mac_st -> 
 			 m_contains (CMA (ilog mac_st.log)) h /\
 		         m_sel h (CMA (ilog mac_st.log)) == Some (l, Buffer.as_seq h tagB)))))
-           (ensures mac_refines i st nonce aad plain cipher h)
+           (ensures mac_refines st nonce aad plain cipher h)
   = ()
- 
+
 #reset-options "--z3timeout 100 --initial_fuel 0 --max_fuel 0 --initial_ifuel 1 --max_ifuel 1"
-let all_above_counterblocks (i:id)
+let rec all_above_counterblocks (i:id{safeId i})
                        (rgn:region)
                        (x:PRF.domain i{ctr_0 i <^ ctr x})
                        (l:nat)
@@ -263,8 +287,16 @@ let all_above_counterblocks (i:id)
                        (to_pos:nat{from_pos <= to_pos /\ to_pos <= l /\ safelen i (to_pos - from_pos) (ctr x)})
                        (plain:Plain.plain i l)
                        (cipher:lbytes l)
-   : Lemma (safeId i ==> (counterblocks i rgn x l from_pos to_pos plain cipher) `all_above` x)
-   = admit() //easy, should do it
+   : Lemma (counterblocks i rgn x l from_pos to_pos plain cipher `all_above` x)
+   = admit ()   
+     (* let remaining = to_pos - from_pos in *)
+     (* if remaining = 0 then *)
+     (*   let _ = counterblocks_lemma i rgn x l from_pos to_pos plain cipher in *)
+     (*   SeqProperties.lemma_contains_empty #(PRF.entry rgn i) *)
+     (* else *)
+     (*   let bl = v (Cipher (blocklen (cipherAlg_of_id i))) in *)
+     (*   let l0 = minNat remaining bl in *)
+     (*   all_above_counterblocks i rgn (PRF.incr i x) l (from_pos + l0) to_pos plain cipher *)
 
 #set-options "--z3timeout 100 --initial_fuel 1 --max_fuel 1 --initial_ifuel 0 --max_ifuel 0"
 let find_cons_hd (#a:Type) (x:a) (tl:Seq.seq a) (f:(a -> Tot bool))
@@ -277,65 +309,65 @@ let contains_intro_2 (#a:Type) (s:Seq.seq a) (x:a) (k:nat)
            ==>
           s `SeqProperties.contains` x)
   = SeqProperties.contains_intro s k x
-  
-#reset-options "--z3timeout 100 --initial_fuel 0 --max_fuel 0 --initial_ifuel 0 --max_ifuel 0"
-let find_mac_counterblocks_none (#rgn:region) (#i:id) (nonce:Cipher.iv (alg i))
-                                (s:Seq.seq (PRF.entry rgn i))
+
+let find_mac_counterblocks_none (#rgn:region) (#i:id) (s:prf_table rgn i)
+                                (nonce:Cipher.iv (alg i))
     : Lemma (requires (s `all_above` (PRF.incr i ({iv=nonce; ctr=ctr_0 i}))))
             (ensures (find_mac s ({iv=nonce; ctr=ctr_0 i}) == None))
-    = admit() //easy, should do it
+    = SeqProperties.lemma_find_l_contains (is_entry_domain ({iv=nonce; ctr=ctr_0 i})) s
 
-val pre_refines_to_refines: (i:id) -> (st:state i Writer) -> (nonce: Cipher.iv (alg i)) ->
-			    (aadlen: UInt32.t {aadlen <=^ aadmax})  ->
-			    (aad: lbuffer (v aadlen)) ->
-                            (len:nat{len<>0}) -> (plain:plainBuffer i len) -> (cipher:lbuffer (len + v MAC.taglen)) ->
-			    (h0:mem) ->
-                            (h:mem{Buffer.live h aad /\ Plain.live h plain /\ Buffer.live h cipher}) 
-   -> Lemma (requires (let mac_rgn = st.prf.mac_rgn in
-     		      let p = Plain.sel_plain h (u len) plain in
-		      let c_tagged = Buffer.as_seq h cipher in
-	              let c, tag = SeqProperties.split c_tagged len in
-		      let ad = Buffer.as_seq h aad in
-  		      safeId i ==> 
-			(none_above ({iv=nonce; ctr=ctr_0 i}) st.prf h0 /\
-   			 pre_refines_one_entry i st nonce len plain cipher h0 h /\
-			 mac_refines i st nonce aad plain cipher h)))
-            (ensures (let mac_rgn = st.prf.mac_rgn in
-     		      let p = Plain.sel_plain h (u len) plain in
-		      let c_tagged = Buffer.as_seq h cipher in
-	              let c, tag = SeqProperties.split c_tagged len in
-		      let ad = Buffer.as_seq h aad in
-  		      let entry = Entry nonce ad len p c_tagged in
-		      safeId i ==>  (
-			pre_refines_one_entry i st nonce len plain cipher h0 h /\ (
-			  let table_0 = HS.sel h0 (PRF.itable i st.prf) in
-			  let table_1 = HS.sel h (PRF.itable i st.prf) in
- 			  let blocks = Seq.slice table_1 (Seq.length table_0) (Seq.length table_1) in
-			  refines_one_entry #mac_rgn #i h entry blocks))))
-#reset-options "--z3timeout 100 --initial_fuel 0 --max_fuel 0 --initial_ifuel 1 --max_ifuel 1"
-let pre_refines_to_refines i st nonce aadlen aad len plain cipher h0 h
-    = if safeId i
-      then let table_0 = HS.sel h0 (PRF.itable i st.prf) in
-      	   let idom = {iv=nonce; ctr=ctr_0 i} in
-	   assert (PRF.find table_0 idom == None);
-	   let table_1 = HS.sel h (PRF.itable i st.prf) in
-  	   let prefix = Seq.slice table_1 0 (Seq.length table_0) in 
-	   assert (Seq.equal prefix table_0);
-	   assert (is_None (find prefix idom));
- 	   let blocks = Seq.slice table_1 (Seq.length table_0) (Seq.length table_1) in
-	   let p = Plain.sel_plain h (u len) plain in
-	   let c_tagged = Buffer.as_seq h cipher in
-           let c, tag = SeqProperties.split c_tagged len in
-	   let hd = Seq.index blocks 0 in
-	   let PRF.Entry x e = hd in
-	   let cbs = counterblocks i st.prf.mac_rgn (PRF.incr i idom) len 0 len p c in
-	   assert (x = idom);
-	   assert (Seq.equal blocks (SeqProperties.cons hd cbs));
-           all_above_counterblocks i st.prf.mac_rgn (PRF.incr i idom) len 0 len p c;
-	   find_mac_counterblocks_none #st.prf.mac_rgn #i nonce cbs;
-	   assert (PRF.is_entry_domain idom hd);
-      	   find_cons_hd hd cbs (PRF.is_entry_domain idom);
-	   find_append idom prefix blocks
+#reset-options "--z3timeout 100 --initial_fuel 0 --max_fuel 0 --initial_ifuel 0 --max_ifuel 0"
+(* val pre_refines_to_refines: (i:id) -> (st:state i Writer) -> (nonce: Cipher.iv (alg i)) -> *)
+(* 			    (aadlen: UInt32.t {aadlen <=^ aadmax})  -> *)
+(* 			    (aad: lbuffer (v aadlen)) -> *)
+(*                             (len:nat{len<>0}) -> (plain:plainBuffer i len) -> (cipher:lbuffer (len + v MAC.taglen)) -> *)
+(* 			    (h0:mem) -> *)
+(*                             (h:mem{Buffer.live h aad /\ Plain.live h plain /\ Buffer.live h cipher})  *)
+(*    -> Lemma (requires (let mac_rgn = st.prf.mac_rgn in *)
+(*      		      let p = Plain.sel_plain h (u len) plain in *)
+(* 		      let c_tagged = Buffer.as_seq h cipher in *)
+(* 	              let c, tag = SeqProperties.split c_tagged len in *)
+(* 		      let ad = Buffer.as_seq h aad in *)
+(*   		      safeId i ==>  *)
+(* 			(none_above ({iv=nonce; ctr=ctr_0 i}) st.prf h0 /\ *)
+(*    			 pre_refines_one_entry i st nonce len plain cipher h0 h /\ *)
+(* 			 mac_refines i st nonce aad plain cipher h))) *)
+(*             (ensures (let mac_rgn = st.prf.mac_rgn in *)
+(*      		      let p = Plain.sel_plain h (u len) plain in *)
+(* 		      let c_tagged = Buffer.as_seq h cipher in *)
+(* 	              let c, tag = SeqProperties.split c_tagged len in *)
+(* 		      let ad = Buffer.as_seq h aad in *)
+(*   		      let entry = Entry nonce ad len p c_tagged in *)
+(* 		      safeId i ==>  ( *)
+(* 			pre_refines_one_entry i st nonce len plain cipher h0 h /\ ( *)
+(* 			  let table_0 = HS.sel h0 (PRF.itable i st.prf) in *)
+(* 			  let table_1 = HS.sel h (PRF.itable i st.prf) in *)
+(*  			  let blocks = Seq.slice table_1 (Seq.length table_0) (Seq.length table_1) in *)
+(* 			  refines_one_entry #mac_rgn #i h entry blocks)))) *)
+(* #reset-options "--z3timeout 100 --initial_fuel 0 --max_fuel 0 --initial_ifuel 1 --max_ifuel 1" *)
+(* let pre_refines_to_refines i st nonce aadlen aad len plain cipher h0 h *)
+(*     = if safeId i *)
+(*       then let table_0 = HS.sel h0 (PRF.itable i st.prf) in *)
+(*       	   let idom = {iv=nonce; ctr=ctr_0 i} in *)
+(* 	   assert (PRF.find table_0 idom == None); *)
+(* 	   let table_1 = HS.sel h (PRF.itable i st.prf) in *)
+(*   	   let prefix = Seq.slice table_1 0 (Seq.length table_0) in  *)
+(* 	   assert (Seq.equal prefix table_0); *)
+(* 	   assert (is_None (find prefix idom)); *)
+(*  	   let blocks = Seq.slice table_1 (Seq.length table_0) (Seq.length table_1) in *)
+(* 	   let p = Plain.sel_plain h (u len) plain in *)
+(* 	   let c_tagged = Buffer.as_seq h cipher in *)
+(*            let c, tag = SeqProperties.split c_tagged len in *)
+(* 	   let hd = Seq.index blocks 0 in *)
+(* 	   let PRF.Entry x e = hd in *)
+(* 	   let cbs = counterblocks i st.prf.mac_rgn (PRF.incr i idom) len 0 len p c in *)
+(* 	   assert (x = idom); *)
+(* 	   assert (Seq.equal blocks (SeqProperties.cons hd cbs)); *)
+(*            all_above_counterblocks i st.prf.mac_rgn (PRF.incr i idom) len 0 len p c; *)
+(* 	   find_mac_counterblocks_none #st.prf.mac_rgn #i nonce cbs; *)
+(* 	   assert (PRF.is_entry_domain idom hd); *)
+(*       	   find_cons_hd hd cbs (PRF.is_entry_domain idom); *)
+(* 	   find_append idom prefix blocks *)
 
 
 (* this version causes a crash *)
@@ -361,8 +393,11 @@ let pre_refines_to_refines i st nonce aadlen aad len plain cipher h0 h
 
 (* 1. empty refines empty *)
 private let refines_empty (h:mem) (i:id{safeId i}) (rgn:region) 
-  : Lemma (refines h i rgn Seq.createEmpty Seq.createEmpty)
-  = ()
+  : Lemma (refines #rgn #i Seq.createEmpty Seq.createEmpty h)
+  = SeqProperties.lemma_contains_empty #(aead_entry i);
+    SeqProperties.lemma_contains_empty #(PRF.entry rgn i);
+    let open FStar.Classical in
+    forall_intro (move_requires (find_mac_counterblocks_none #rgn #i Seq.createEmpty))
 
 (* block_lengths: used only for the statement of the next lemma *)
 private let rec block_lengths (#i:id{safeId i}) (entries:Seq.seq (entry i)) 
